compcertox/KRel.v
@@ -1,0 +1,111 @@
+From Coq Require Import
+     Relations RelationClasses List.
+From compcertox Require Import
+     Lifting AbstractStateRel.
+From compcert.lib Require Import
+     Coqlib.
+From compcert.common Require Import
+     LanguageInterface Events
+     Globalenvs Smallstep
+     Linking Memory Values.
+From compcert.cklr Require Import
+     CKLR Extends Clightrel.
+From compcert.cfrontend Require Import
+     SimplLocalsproof Clight.
+
+Definition blocks (se: Genv.symtbl) (names: ident -> Prop) : block -> Z -> Prop :=
+  fun b ofs => exists v, names v /\ Genv.find_symbol se v = Some b.
+
+(** The relation Rr is parametrized by the symbol table so that we do not have
+    to bind the variables being abstracted to particular blocks *)
+Record krel {K1 K2: Type}: Type :=
+  mk_krel {
+      krel_rel (se: Genv.symtbl):> K2 -> mem * K1 -> Prop;
+      (** the names of the static variables being abstracted *)
+      vars : ident -> Prop;
+      (** other variables *)
+      others := fun i => ~ vars i;
+
+      (** the abstraction relation is not affected by other variables *)
+      G_unchanged: forall se k1 k2 m m',
+        krel_rel se k2 (m, k1) -> Mem.unchanged_on (blocks se vars) m m' -> krel_rel se k2 (m', k1);
+      (** the abstraction relation only focuses on valid blocks, i.e. those have
+          been allocated *)
+      G_valid: forall se k1 k2 m b ofs,
+        krel_rel se k2 (m, k1) -> (blocks se vars) b ofs -> Mem.valid_block m b;
+    }.
+Arguments krel: clear implicits.
+
+Section KREL_KCC.
+
+  Context {K1 K2} (R: krel K2 K1).
+  Context (se: Genv.symtbl).
+
+  Inductive krel_kcc_query: query (li_c @ K1) -> query (li_c @ K2) -> Prop :=
+    krel_kcc_query_intro vf1 vf2 sg vargs1 vargs2 m1 m2 k1 k2:
+      Val.inject inject_id vf1 vf2 -> Val.inject_list inject_id vargs1 vargs2 ->
+      Mem.extends m1 m2 -> vf1 <> Vundef -> no_perm_on m1 (blocks se (vars R)) ->
+      krel_rel R se k1 (m2, k2) ->
+      krel_kcc_query (cq vf1 sg vargs1 m1, k1) (cq vf2 sg vargs2 m2, k2).
+  Inductive krel_kcc_reply: reply (li_c @ K1) -> reply (li_c @ K2) -> Prop :=
+    krel_kcc_reply_intro vres1 m1 vres2 m2 k1 k2:
+      Val.inject inject_id vres1 vres2 ->
+      Mem.extends m1 m2 -> no_perm_on m1 (blocks se (vars R)) ->
+      krel_rel R se k1 (m2, k2) ->
+      krel_kcc_reply (cr vres1 m1, k1) (cr vres2 m2, k2).
+
+  (* Instance symtbl_kf: KripkeFrame unit Genv.symtbl := *)
+  (*   {| acc _ := eq; |}. *)
+
+  Program Definition krel_kcc: callconv (li_c @ K1) (li_c @ K2) :=
+    {|
+      ccworld := unit;
+      match_senv _ := eq;
+      match_query _ := krel_kcc_query;
+      match_reply _ := krel_kcc_reply;
+    |}.
+  Next Obligation.
+    inv H0. cbn. apply val_inject_id in H4. inv H4; easy.
+  Qed.
+  Next Obligation.
+    inv H. cbn. apply val_inject_id in H4. inv H4; easy.
+  Qed.
+
+End KREL_KCC.
+
+Ltac unchanged_implies_solve:=
+  eapply Mem.unchanged_on_implies; [eauto | intros b ofs [v [? ?]]; eexists; eauto].
+
+Section COMP.
+
+  (* TODO: Do we need the assumption that R and S do not overlap *)
+  Context {K1 K2 K3} (R: krel K1 K2) (S: krel K2 K3).
+
+  Local Obligation Tactic := cbn.
+  (* TODO: Promoting to callconv preserves composition *)
+  Program Definition krel_comp: krel K1 K3 :=
+    {|
+      krel_rel se :=
+        fun k3 '(m1, k1) => exists k2, S se k3 (m1, k2) /\ R se k2 (m1, k1);
+      vars i := vars S i \/ vars R i;
+    |}.
+  Next Obligation.
+    intros se k1 k3 m1 m1' (k2 & HS & HR) H.
+    eexists k2. split.
+    - eapply G_unchanged; eauto.
+      unchanged_implies_solve.
+    - eapply G_unchanged; eauto.
+      unchanged_implies_solve.
+  Qed.
+  Next Obligation.
+    intros se k1 k3 * (k2 & HS & HR) Hb.
+    unfold blocks in Hb. destruct Hb as (v & Hv & ?).
+    destruct Hv.
+    - eapply G_valid. apply HS.
+      exists v; split; auto.
+    - eapply G_valid. apply HR.
+      exists v; split; auto.
+      Unshelve. apply ofs. apply ofs.
+  Qed.
+
+End COMP.
